Some safe signed integer

safe_int/SafeInt.thy
@@ -1,7 +1,44 @@
 theory SafeInt
 
-imports Main
+imports Main "~~/src/HOL/Word/Word" 
 
 begin
+
+(* signed 32 bit *)
+
+type_synonym int32 = "32 word"
+
+datatype safeInt32 = Invalid | Data "int32"
+
+(* When does a safeInt32 represent an int *)
+(* Note: int is the type of arbitrary precision integers. *)
+
+fun represent :: "safeInt32 \<Rightarrow> int \<Rightarrow> bool"
+  where
+  "represent Invalid _ = True"
+| "represent (Data d) i = (sint d = i)"
+
+definition sadd_test :: "int32 \<Rightarrow> int32 \<Rightarrow> bool"
+  where "sadd_test x y = ((x + y XOR x) AND (x + y XOR y) >> size x - 1 = 0)"
+
+lemma sadd_test_sound :
+  "sadd_test x y \<Longrightarrow> sint x + sint y = sint (x + y)"
+  by(simp add: sadd_test_def  Word.sofl_test)
+
+fun add :: "safeInt32 \<Rightarrow> safeInt32 \<Rightarrow> safeInt32"
+  where
+  "add Invalid _ = Invalid"
+| "add _ Invalid = Invalid"
+| "add (Data a) (Data b) =
+     (if sadd_test a b then Data (a + b) else Invalid)"
+
+lemma add_good :
+  "represent a x \<Longrightarrow>
+   represent b y \<Longrightarrow>
+   represent (add a b) (x + y)"
+  apply(cases a; auto)
+  apply(cases b; auto)
+  apply(rename_tac c d)
+  by(simp add: sadd_test_sound)
 
 end
